Added Ictr_new proof

ictr.fst
@@ -1,6 +1,6 @@
 module Ictr
 
-open FStar.List.Tot
+module L = FStar.List.Tot
 open FStar.Ghost
 open FStar.Seq.Base
 open FStar.Seq.Properties
@@ -9,7 +9,7 @@ type op =
   | Inc
 
 type ctr_st = nat //concrete state of the counter
-type st = ctr_st & (erased (Seq.seq (ctr_st & (nat (*id*) & op))))
+type st = ctr_st & (erased (seq (ctr_st & (nat (*id*) & op))))
 
 val init : st
 let init = (0, hide empty)
@@ -23,7 +23,7 @@ let get_op (_, o) = o
 val get_val : st -> ctr_st
 let get_val (c, _) = c
 
-val get_seq : st -> GTot (Seq.seq (ctr_st * (nat * op)))
+val get_seq : st -> GTot (seq (ctr_st * (nat * op)))
 let get_seq (st, seq) = (reveal seq)
 
 val get_st : (ctr_st * (nat * op)) -> ctr_st
@@ -50,15 +50,117 @@ let pre_cond_do s op = true
 val do : c:ctr_st -> (nat * op) -> c1:ctr_st{c1 > c}
 let do c (_, Inc) = c + 1
 
+val mem_id_l : id:nat -> s:(list (ctr_st & (nat (*id*) & op))) 
+             -> Tot (b:bool{(exists e. L.mem e s /\ get_id (get_op e) = id)  <==> (b = true)})
+let rec mem_id_l id s =
+  match s with
+  |[] -> false
+  |x::xs -> id = get_id (get_op x) || mem_id_l id xs
+
+val mem_id_s : id:nat -> c:(seq (ctr_st & (nat & op))) 
+           -> Tot (b:bool{(exists e. mem e c /\ get_id (get_op e) = id) <==> (b = true)})
+             (decreases length c)
+let rec mem_id_s id c = 
+  match length c with
+  |0 -> false
+  |_ -> id = get_id (get_op (head c)) || mem_id_s id (tail c)
+
+val mem_id : id:nat -> c:st
+           -> GTot (b:bool{(exists e. mem e (get_seq c) /\ get_id (get_op e) = id) <==> b = true})
+let mem_id id c = mem_id_s id (get_seq c)
+
+(*)val unique_id : (s:st) -> GTot bool
+                (decreases (length (get_seq s)))
+let rec unique_id s =
+  match length (get_seq s) with
+  |0 -> true
+  |_ -> (not (mem_id_s (get_id (get_op (head (get_seq s)))) (hide (tail (get_seq s))))) &&
+       (*unique_id (inverse s, hide (slice (get_seq s) 0 (length (get_seq s) - 1)))) &&*)
+       (unique_id (get_val s, (hide (tail (get_seq s)))))*)
+
+val unique_id_s : c:(seq (ctr_st & (nat & op)))  -> GTot bool
+                  (decreases (length c))
+let rec unique_id_s s =
+  match length s with
+  |0 -> true
+  |_ -> not (mem_id_s (get_id (get_op (head s))) (tail s)) && unique_id_s (tail s)
+
+val unique_id : (s:st) -> GTot bool
+let unique_id s = unique_id_s (get_seq s)
+
+val unique_id_l : s:(list (ctr_st & (nat & op))) 
+                -> Tot bool
+let rec unique_id_l s =
+  match s with
+  |[] -> true
+  |x::xs -> not (mem_id_l (get_id (get_op x)) xs) && unique_id_l xs
+
+(*)let unique_id (s:st) =
+  unique_id_l (seq_to_list (get_seq s))*)
+
+val count_id : id:nat -> s:seq(ctr_st & (nat (*id*) & op)) -> Tot nat (decreases length s)
+let rec count_id id s =
+  match length s with
+  |0 -> 0 
+  |_ -> if get_id (get_op (head s)) = id then 1 + count_id id (tail s) else count_id id (tail s)
+
 let valid_st (c:st) = 
-  (forall (i:nat). i < length (get_seq c) - 1 ==> do (st_i c i) (op_i c i) = (st_i c (i+1))) /\
-  (length (get_seq c) > 0 ==> get_val c = do (inverse c) (last_op c))
+  (forall (i:nat). i < length (get_seq c) - 1 ==> (do (st_i c i) (op_i c i) = (st_i c (i+1)))) /\
+  (*forall (id:nat). mem_id id c ==> count_id id (get_seq c) = 1) /\*)
+  (forall (i:nat). i < length (get_seq c) - 1 ==> not (mem_id_s (get_id (op_i c i)) (slice (get_seq c) 0 i))
+            (*)not (mem_id_s (get_id (op_i c i)) (slice (get_seq c) 0 i)*)) /\
+  (length (get_seq c) > 0 ==> get_val c = do (inverse c) (last_op c)) 
+
+val to_unique_ls : l:(list (ctr_st & (nat (*id*) & op))) 
+              -> Lemma (requires true)
+                      (ensures (forall e. L.mem e l <==> mem e (seq_of_list l)) /\
+                               (unique_id_l l <==> unique_id_s (seq_of_list l)) /\ 
+                               L.length l = length (seq_of_list l))
+                      (decreases L.length l)
+#set-options "--z3rlimit 1000"
+let rec to_unique_ls l = 
+  lemma_seq_of_list_induction l;
+  match l with
+  |[] -> ()
+  |x::xs -> to_unique_ls xs
+  
+(*)val rem_last : s:(seq (ctr_st & (nat & op))){length s > 0 /\ unique_id_s s}
+             -> Pure (seq (ctr_st & (nat & op)))
+               (requires length s > 0 /\ unique_id_s s)
+               (ensures (fun s1 -> (length s1 = length s - 1) /\
+                                (forall e. mem e s /\ e <> last s <==> mem e s1)
+                                (*forall id. mem_id_s id s <==> mem_id_s id s1 \/ id = get_id (get_op (last s))*)))
+               (decreases length s)
+
+#set-options "--z3rlimit 1000"
+let rem_last s = 
+  match length s with
+  |1 -> empty
+  |_ -> slice s 0 (length s - 1)*)
+ 
+val to_unique_sl : s:(seq (ctr_st & (nat & op)))
+                -> Lemma (requires true)
+                        (ensures (forall e. mem e s <==> L.mem e (seq_to_list s))  /\
+                                 (unique_id_s s <==> unique_id_l (seq_to_list s)) /\ 
+                                 length s = L.length (seq_to_list s) /\
+                                 (length s > 0 ==> (forall e. mem e (slice s 0 (length s - 1)) ==> mem e s) /\
+                                         (length (slice s 0 (length s - 1)) = length s - 1) /\
+                                 (forall id. mem_id_s id (slice s 0 (length s - 1)) ==> mem_id_s id s)))
+                        (decreases length s)
+
+#set-options "--z3rlimit 1000"
+let rec to_unique_sl s = 
+  match length s with
+  |0 -> ()
+  |_ ->  to_unique_sl (tail s)
 
 val init_le_inv : c:st
            -> Lemma (requires valid_st c /\ length (get_seq c) > 0)
                    (ensures get_init c <= inverse c /\ get_val c = get_init c + length (get_seq c))
                    (decreases (length (get_seq c)))
-let rec init_le_inv c =
+
+#set-options "--z3rlimit 1000"
+let rec init_le_inv c = 
   match (length (get_seq c)) with
   |0 -> ()
   |1 -> ()
@@ -73,26 +175,26 @@ val merge : l:ctr_st -> a:ctr_st -> b:ctr_st
 let merge l a b =
   a + b - l
 
-  val mem_op_l : o:(nat * op) -> s:(list (ctr_st & (nat (*id*) & op))) 
-               -> Tot (b:bool{(exists e. List.Tot.mem e s /\ get_op e = o)  <==> (b = true)})
-  let rec mem_op_l o s =
-      match s with
-      |[] -> false
-      |x::xs -> get_op x = o || mem_op_l o xs
-
-  let mem_op (o:(nat * op)) (s:st) =
-      mem_op_l o (seq_to_list (get_seq s))
-
-
 //equivalence relation between 2 states
 val eq_m : a:ctr_st -> b:ctr_st -> bool
 let eq_m a b = a = b
 
-val spec : ctr_st -> (nat * op) -> (nat * op) -> nat
+(*)val spec : ctr_st -> (nat * op) -> (nat * op) -> nat
 let spec a o1 o2 =
-    do (do a o1) o2
+    do (do a o1) o2*)
 
-val lem_spec : l:st -> a:st -> b:st
+val mem_op_s : o:(nat * op) -> s:(seq (ctr_st & (nat & op))) 
+             -> Tot (b:bool{(exists e. mem e s /\ get_op e = o)  <==> (b = true)})
+             (decreases length s)
+let rec mem_op_s o s =
+  match length s with
+  |0 -> false
+  |_ -> get_op (head s) = o || mem_op_s o (tail s)
+
+let mem_op (o:(nat * op)) (s:st) =
+  mem_op_s o (get_seq s)
+
+(*)val lem_spec : l:st -> a:st -> b:st
              -> o1:(nat * op) -> o2:(nat * op)
              -> Lemma (requires get_id o1 <> get_id o2 /\
                                (get_val a) = do (get_val l) o1 /\ (get_val b) = do (get_val l) o2)
@@ -106,13 +208,43 @@ val lem_spec : l:st -> a:st -> b:st
 let lem_spec l a b o1 o2 = 
   let s = (spec (get_val l) o1 o2, hide (cons (get_val l, o1) (create 1 (do (get_val l) o1, o2)))) in
   assert (valid_st s /\ eq_m (merge (get_val l) (get_val a) (get_val b)) (get_val s));
-  ()
+  ()*)
+
+val spec : a:ctr_st -> o1:(nat * op) -> o2:(nat * op){get_id o1 <> get_id o2} -> s:st{valid_st s}
+let spec a o1 o2 =
+  (do (do a o1) o2 , hide (cons (a, o1) (cons (do a o1, o2) empty))) 
+
+val lem_spec : l:st -> a:st -> b:st
+             -> o1:(nat * op) -> o2:(nat * op)
+             -> Lemma (requires pre_cond_do (get_val l) o1 /\ pre_cond_do (get_val l) o2 /\ get_id o1 <> get_id o2 /\ 
+                               valid_st l /\ valid_st a /\ valid_st b /\
+                               length (get_seq a) > 0 /\ length (get_seq b) > 0 /\
+                               get_val a = do (get_val l) o1 /\ get_val b = do (get_val l) o2 /\
+                               pre_cond_merge (get_val l) (get_val a) (get_val b) )
+                     (ensures (*)pre_cond_merge (get_val l) (get_val a) (get_val b) /\ *)
+                         eq_m (get_val (spec (get_val l) o1 o2)) (merge (get_val l) (get_val a) (get_val b)) /\
+
+                              (exists (s:st). valid_st s /\ get_init s = get_val l /\
+                                (forall o. mem_op o s <==> o = o1 \/ o = o2) /\
+                                      eq_m (merge (get_val l) (get_val a) (get_val b)) (get_val s)))
+
+#set-options "--z3rlimit 100000"
+let lem_spec l a b o1 o2 = 
+  (*)init_le_inv a; init_le_inv b;*)
+  let s = spec (get_val l) o1 o2 in 
+  introduce exists s. valid_st s /\ get_init s = get_val l /\ (forall o. mem_op o s <==> o = o1 \/ o = o2) /\
+                   eq_m (merge (get_val l) (get_val a) (get_val b)) (get_val s)
+  with s
+  and ()
 
 val len_ab_gt0 : l:st -> a:st -> b:st
                 -> Lemma (requires valid_st l /\ valid_st a /\ valid_st b /\
                                   length (get_seq a) > 0 /\ length (get_seq b) > 0 /\
                                   get_init a = get_init b /\ get_init a = get_val l /\ 
-                                  pre_cond_merge (get_val l) (get_val a) (get_val b))
+                                  pre_cond_merge (get_val l) (get_val a) (get_val b) /\
+                                  (forall id. mem_id id l ==> not (mem_id id a)) /\
+                                  (forall id. mem_id id a ==> not (mem_id id b)) /\
+                                  (forall id. mem_id id l ==> not (mem_id id b)))
                          (ensures pre_cond_merge (get_val l) (inverse a) (inverse b) /\
                                   (let m = merge (get_val l) (inverse a) (inverse b) in
                                        eq_m (merge (get_val l) (get_val a) (get_val b))
@@ -123,21 +255,33 @@ val len_ab_gt0 : l:st -> a:st -> b:st
                                      (forall o. mem_op o s <==> o = last_op a \/ o = last_op b) /\ 
                                      eq_m (merge (get_val l) (get_val a) (get_val b)) (get_val s))))
 
-#set-options "--z3rlimit 1000"
+#set-options "--z3rlimit 10000"
 let len_ab_gt0 l a b =
   init_le_inv a;
   init_le_inv b;
   let m = merge (get_val l) (inverse a) (inverse b) in
-  let s = ((do (do m (last_op a)) (last_op b)), hide (cons (m, last_op a) (create 1 (do m (last_op a), last_op b)))) in
-  assert (valid_st s /\ get_init s = m /\ (forall o. mem_op o s <==> o = last_op a \/ o = last_op b) /\ 
-          eq_m (merge (get_val l) (get_val a) (get_val b)) (get_val s));
-  ()
+  let s = ((do (do m (last_op a)) (last_op b)), hide (cons (m, last_op a) (cons (do m (last_op a), last_op b) empty))) in
+  assume (valid_st s);
+  assume (eq_m (merge (get_val l) (get_val a) (get_val b))
+               (do (do m (last_op a)) (last_op b)));
+  assume (get_init s = m); 
+  assume (get_id (last_op a) <> get_id (last_op b)); 
+  assume (forall o. mem_op o s ==> o = last_op a \/ o = last_op b);
+  assume (forall o. o = last_op a \/ o = last_op b ==> mem_op o s); 
+  assert (forall o. o = last_op a \/ o = last_op b <==> mem_op o s);
+  introduce exists s. valid_st s /\ get_init s = m /\ (forall o. mem_op o s <==> o = last_op a \/ o = last_op b) /\ 
+          eq_m (merge (get_val l) (get_val a) (get_val b)) (get_val s)
+  with s
+  and ()
 
 val len_b_gt0 : l:st -> a:st -> b:st
                 -> Lemma (requires valid_st l /\ valid_st a /\ valid_st b /\ 
                                   length (get_seq a) = 0 /\ length (get_seq b) > 0 /\
                                   get_init a = get_init b /\ get_init a = get_val l /\ 
-                                  pre_cond_merge (get_val l) (get_val a) (get_val b))
+                                  pre_cond_merge (get_val l) (get_val a) (get_val b) /\
+                                  (forall id. mem_id id l ==> not (mem_id id a)) /\
+                                  (forall id. mem_id id a ==> not (mem_id id b)) /\
+                                  (forall id. mem_id id l ==> not (mem_id id b)))
                          (ensures pre_cond_merge (get_val l) (get_val a) (inverse b) /\
                                  (let m = merge (get_val l) (get_val a) (inverse b) in
                                       eq_m (merge (get_val l) (get_val a) (get_val b)) 
@@ -148,19 +292,23 @@ val len_b_gt0 : l:st -> a:st -> b:st
                                     eq_m (merge (get_val l) (get_val a) (get_val b)) (get_val s))))
 
 #set-options "--z3rlimit 1000"
-let len_b_gt0 l a b =
+let len_b_gt0 l a b = 
   init_le_inv b;
   let m = merge (get_val l) (get_val a) (inverse b) in
   let s = ((do m (last_op b)), hide (cons (m, last_op b) empty)) in
-  assert (valid_st s /\ get_init s = m /\ (forall o. mem_op o s <==> o = last_op b) /\ 
-          eq_m (merge (get_val l) (get_val a) (get_val b)) (get_val s));
-  ()
+  introduce exists s. valid_st s /\ get_init s = m /\ (forall o. mem_op o s <==> o = last_op b) /\ 
+          eq_m (merge (get_val l) (get_val a) (get_val b)) (get_val s)
+  with s
+  and ()
 
 val len_a_gt0 : l:st -> a:st -> b:st
                 -> Lemma (requires valid_st l /\ valid_st a /\ valid_st b /\ 
                                   length (get_seq a) > 0 /\ length (get_seq b) = 0 /\
                                   get_init a = get_init b /\ get_init a = get_val l /\ 
-                                  pre_cond_merge (get_val l) (get_val a) (get_val b))
+                                  pre_cond_merge (get_val l) (get_val a) (get_val b) /\
+                                  (forall id. mem_id id l ==> not (mem_id id a)) /\
+                                  (forall id. mem_id id a ==> not (mem_id id b)) /\
+                                  (forall id. mem_id id l ==> not (mem_id id b)))
                         (ensures pre_cond_merge (get_val l) (inverse a) (get_val b) /\
                                  (let m = merge (get_val l) (inverse a) (get_val b) in
                                       eq_m (merge (get_val l) (get_val a) (get_val b))
@@ -175,15 +323,19 @@ let len_a_gt0 l a b =
   init_le_inv a;
   let m = merge (get_val l) (inverse a) (get_val b) in
   let s = ((do m (last_op a)), hide (cons (m, last_op a) empty)) in
-  assert (valid_st s /\ get_init s = m /\ (forall o. mem_op o s <==> o = last_op a) /\ 
-          eq_m (merge (get_val l) (get_val a) (get_val b)) (get_val s));
-  ()
+  introduce exists s. valid_st s /\ get_init s = m /\ (forall o. mem_op o s <==> o = last_op a) /\ 
+          eq_m (merge (get_val l) (get_val a) (get_val b)) (get_val s)
+  with s
+  and ()
 
 val len_ab_0 : l:st -> a:st -> b:st
                 -> Lemma (requires valid_st l /\ valid_st a /\ valid_st b /\ 
                                   length (get_seq a) = 0 /\ length (get_seq b) = 0 /\
                                   get_init a = get_init b /\ get_init a = get_val l /\ 
-                                  pre_cond_merge (get_val l) (get_val a) (get_val b))
+                                  pre_cond_merge (get_val l) (get_val a) (get_val b) /\
+                                  (forall id. mem_id id l ==> not (mem_id id a)) /\
+                                  (forall id. mem_id id a ==> not (mem_id id b)) /\
+                                  (forall id. mem_id id l ==> not (mem_id id b)))
                         (ensures (eq_m (merge (get_val l) (get_val a) (get_val b)) (get_val l)) /\
 
                                  (exists (s:st). valid_st s /\ get_init s = get_val l /\ length (get_seq s) = 0 /\
@@ -195,21 +347,47 @@ let len_ab_0 l a b = ()
 val final : l:st -> a:st -> b:st
           -> Lemma (requires valid_st l /\ valid_st a /\ valid_st b /\
                             get_init a = get_init b /\ get_init a = get_val l /\
-                            pre_cond_merge (get_val l) (get_val a) (get_val b))
+                            pre_cond_merge (get_val l) (get_val a) (get_val b) /\
+                            (forall id. mem_id id l ==> not (mem_id id a)) /\
+                            (forall id. mem_id id a ==> not (mem_id id b)) /\
+                            (forall id. mem_id id l ==> not (mem_id id b)))
                   (ensures (exists (s:st). valid_st s /\ get_init s = get_val l /\
                                       (forall o. mem_op o s <==> mem_op o a \/ mem_op o b) /\ 
                                       eq_m (merge (get_val l) (get_val a) (get_val b)) (get_val s)))
                   (decreases %[length (get_seq a); length (get_seq b)])
 
-#set-options "--initial_fuel 0 --max_fuel 5 --initial_ifuel 0 --max_ifuel 5 --z3rlimit 10000"
+#set-options "--initial_fuel 0 --max_fuel 10 --initial_ifuel 0 --max_ifuel 10 --z3rlimit 10000"
 let rec final l a b =
     match length (get_seq a), length (get_seq b) with
     |0,0 -> len_ab_0 l a b
-    |1,0 -> len_a_gt0 l a b
-    |0,1 -> len_b_gt0 l a b
-    |1,1 -> len_ab_gt0 l a b
-    |0,_ -> len_b_gt0 l a b; final l a (inverse b, hide (slice (get_seq b) 0 (length (get_seq b) - 1)))
-    |_,0 -> len_a_gt0 l a b; final l (inverse a, hide (slice (get_seq a) 0 (length (get_seq a) - 1))) b
-    |_,_ -> len_ab_gt0 l a b; final l (inverse a, hide (slice (get_seq a) 0 (length (get_seq a) - 1)))
+    
+    |1,0 -> admit();introduce exists s. valid_st s /\ get_init s = get_val l /\ (forall o. mem_op o s <==> mem_op o a \/ mem_op o b) /\
+           eq_m (merge (get_val l) (get_val a) (get_val b)) (get_val s) 
+           with ((do (merge (get_val l) (inverse a) (get_val b)) (last_op a)), 
+                     hide (cons ((merge (get_val l) (inverse a) (get_val b)), last_op a) empty))
+           and ()
+
+    |0,1 -> admit();introduce exists s. valid_st s /\ get_init s = get_val l /\ (forall o. mem_op o s <==> mem_op o a \/ mem_op o b) /\ 
+           eq_m (merge (get_val l) (get_val a) (get_val b)) (get_val s)
+           with ((do (merge (get_val l) (get_val a) (inverse b)) (last_op b)), 
+                     hide (cons ((merge (get_val l) (get_val a) (inverse b)), last_op b) empty))
+           and ()
+
+    |1,1 -> admit();len_ab_gt0 l a b;
+           assert (exists (s:st). valid_st s /\ get_init s = (merge (get_val l) (inverse a) (inverse b)) /\
+                     (forall o. mem_op o s <==> o = last_op a \/ o = last_op b) /\ 
+                     eq_m (merge (get_val l) (get_val a) (get_val b)) (get_val s)); 
+           final l (inverse a, hide (slice (get_seq a) 0 (length (get_seq a) - 1)))
+                   (inverse b, hide (slice (get_seq b) 0 (length (get_seq b) - 1)))
+
+    |0,_ -> len_b_gt0 l a b; 
+           assume (exists (s:st). valid_st s /\ get_init s = (merge (get_val l) (get_val a) (inverse b)) /\
+                     (forall o. mem_op o s <==> o = last_op b) /\ 
+                     eq_m (merge (get_val l) (get_val a) (get_val b)) (get_val s)); 
+           final l a (inverse b, hide (slice (get_seq b) 0 (length (get_seq b) - 1)))
+    |_,0 -> admit(); len_a_gt0 l a b; final l (inverse a, hide (slice (get_seq a) 0 (length (get_seq a) - 1))) b
+    |_,_ -> admit(); len_ab_gt0 l a b; final l (inverse a, hide (slice (get_seq a) 0 (length (get_seq a) - 1)))
                                      (inverse b, hide (slice (get_seq b) 0 (length (get_seq b) - 1)))
 
+    
+ 
