ictr_new.fst
@@ -1,0 +1,253 @@
+module Ictr_new
+
+open FStar.Seq
+open FStar.Ghost
+
+// the concrete state type
+// e.g. for the increment only counter (icounter), concrete_st = nat
+type concrete_st = nat
+
+// operation type
+// (the only operation is increment, so unit is fine)
+type op_t = unit
+
+type timestamp_t = nat
+
+type log_entry = timestamp_t & op_t
+
+type log = seq log_entry
+
+unfold
+  let ( ++ ) (l1 l2:log) = Seq.append l1 l2
+
+let distinct_ops (l:log) : prop = forall (e:log_entry). count e l <= 1
+
+let distinct_invert_append (a b:log)
+  : Lemma
+      (requires distinct_ops (a ++ b))
+      (ensures distinct_ops a /\ distinct_ops b)
+      [SMTPat (distinct_ops (a ++ b))]
+  = lemma_append_count a b
+
+type st0 = concrete_st & erased (concrete_st & log)
+
+let v_of (s:st0) : concrete_st = fst s
+let init_of (s:st0) : GTot concrete_st = fst (snd s)
+let ops_of (s:st0) : GTot log = snd (snd s)
+
+let rec seq_foldl (f:concrete_st -> log_entry -> concrete_st) (x:concrete_st) (s:seq log_entry)
+  : Tot concrete_st (decreases Seq.length s)
+  = if Seq.length s = 0 then x
+       else let hd, tl = Seq.head s, Seq.tail s in
+            seq_foldl f (f x hd) tl
+
+// apply an operation to a state
+let do (s:concrete_st) (o:log_entry) : (r:concrete_st{r = s + 1}) = s + 1
+
+let valid_st (s:st0) : prop =
+  (*)distinct_ops (ops_of s) /\*)
+  v_of s == seq_foldl do (init_of s) (ops_of s)
+
+type st = s:st0{valid_st s}
+
+let rec lem_foldl (s:concrete_st) (l:log) 
+  : Lemma (ensures (seq_foldl do s l) = s + length l) (decreases length l)
+  = match length l with
+    |0 -> ()
+    |_ -> lem_foldl (do s (head l)) (tail l)
+
+let linearized_merge (s:concrete_st) (l:log) : (r:st{v_of r = seq_foldl do s l}) =
+  let r = (seq_foldl do s l, hide (s,l)) in
+  lem_foldl s l; r
+
+//conflict resolution
+let resolve_conflict (x y:log_entry) : log =
+  cons x (cons y empty)
+
+let resolve_conflict_len (x y:log_entry)
+  : Lemma (Seq.length (resolve_conflict x y) = 2)
+  = ()
+
+let is_x_or_y (#a:Type) (s:seq a{Seq.length s == 1}) (x y : a) =
+  Seq.index s 0 == x \/ Seq.index s 0 == y
+
+let is_x_and_y (#a:Type) (s:seq a{Seq.length s == 2}) (x y : a) =
+  (Seq.index s 0 == x /\ Seq.index s 1 == y) \/
+  (Seq.index s 0 == y /\ Seq.index s 1 == x)
+
+let resolve_conflict_mem (x y:log_entry)
+  : Lemma (resolve_conflict_len x y;
+           let s = resolve_conflict x y in
+           (Seq.length s == 1 ==> is_x_or_y s x y) /\
+           (Seq.length s == 2 ==> is_x_and_y s x y))
+  = ()
+
+
+#set-options "--query_stats"
+// l is interleaving of l1 and l2
+let rec is_interleaving (l l1 l2:log) 
+  : Tot Type0 (decreases %[Seq.length l1; Seq.length l2]) =
+
+  // l1 and l2 are empty
+    ((Seq.length l1 == 0 /\ Seq.length l2 == 0) ==> l == empty) 
+
+    /\
+
+  // if l1 is empty, then l == l2
+  (Seq.length l1 == 0 /\ Seq.length l2 <> 0 ==> l == l2)
+
+  /\
+
+  // similarly for l2 being empty
+  (Seq.length l2 == 0 /\ Seq.length l1 <> 0 ==> l == l1)
+
+  /\
+
+  // length of l1 and l2 = 1
+  ((Seq.length l1 = 1 /\ Seq.length l2 = 1) ==>
+
+    l == (resolve_conflict (last l1) (last l2)))
+
+  /\
+
+  // if both are non-empty and lengths > 1
+  // then three cases
+  ((Seq.length l1 > 1 /\ Seq.length l2 > 1) ==>
+
+   (let prefix1, last1 = un_snoc l1 in
+    let prefix2, last2 = un_snoc l2 in
+
+    (exists l'. is_interleaving l' prefix1 prefix2 /\
+           l == l' ++ (resolve_conflict last1 last2))
+
+    \/
+
+    (exists l'. is_interleaving l' l1 prefix2 /\
+           l == Seq.snoc l' last2)
+
+    \/
+
+    (exists l'. is_interleaving l' prefix1 l2 /\
+           l == Seq.snoc l' last1)))
+
+// concrete merge pre-condition
+let concrete_merge_pre (lca a b:concrete_st) : prop
+  = a >= lca /\ b >= lca
+
+// concrete merge operation
+let concrete_merge (lca:concrete_st) (cst1:concrete_st) (cst2:concrete_st{concrete_merge_pre lca cst1 cst2}) 
+  : concrete_st = cst1 + cst2 - lca
+
+let inverse (s:st{length (ops_of s) <> 0}) 
+          : GTot (r:concrete_st{let p, l = un_snoc (ops_of s) in
+                      (r == seq_foldl do (init_of s) p)})
+    = let p, l = un_snoc (ops_of s) in
+      let r = seq_foldl do (init_of s) p in
+      r
+
+let rec lem_inverse (s:st)
+  : Lemma (requires length (ops_of s) <> 0)
+          (ensures (v_of s == do (inverse s) (last (ops_of s))) /\
+                   (inverse s >= init_of s) /\ (v_of s = init_of s + length (ops_of s)) /\ (v_of s >= init_of s))
+          (decreases length (ops_of s))
+  = match length (ops_of s) with
+    |0 -> ()
+    |1 -> ()
+    |_ -> lem_inverse (seq_foldl do (do (init_of s) (head (ops_of s))) (tail (ops_of s)),
+                     (hide (do (init_of s) (head (ops_of s)), (tail (ops_of s)))))
+
+
+// length of both branches is > 0
+#set-options "--z3rlimit 1000"
+let linearizable_ab_gt0 (lca a b:st)
+  : Lemma
+      (requires 
+          length (ops_of a) <> 0 /\ length (ops_of b) <> 0 /\
+          v_of lca == init_of a /\
+          init_of a == init_of b)
+      (ensures 
+         concrete_merge_pre (v_of lca) (v_of a) (v_of b) /\
+         concrete_merge_pre (v_of lca) (inverse a) (inverse b) /\
+         (let inv = concrete_merge (v_of lca) (inverse a) (inverse b) in
+            concrete_merge (v_of lca) (v_of a) (v_of b) =
+            seq_foldl do inv (resolve_conflict (last (ops_of a)) (last (ops_of b))) /\
+            (exists l. is_interleaving l (cons (last (ops_of a)) empty ) (cons (last (ops_of b)) empty) /\
+                  v_of (linearized_merge inv l) == concrete_merge (v_of lca) (v_of a) (v_of b))))
+  = lem_inverse a;
+    lem_inverse b;
+    assert (length (cons (last (ops_of a)) empty) = 1 /\ length (cons (last (ops_of b)) empty) = 1);
+    assert (is_interleaving (resolve_conflict (last (cons (last (ops_of a)) empty)) 
+                                              (last (cons (last (ops_of b)) empty)))
+                            (cons (last (ops_of a)) empty) (cons (last (ops_of b)) empty));()
+
+
+// length of branch a is > 0 and branch b is 0
+let linearizable_a_gt0 (lca a b:st)
+  : Lemma
+      (requires 
+         length (ops_of a) <> 0 /\ length (ops_of b) = 0 /\
+         v_of lca == init_of a /\
+         init_of a == init_of b)
+      (ensures 
+         concrete_merge_pre (v_of lca) (v_of a) (v_of b) /\
+         concrete_merge (v_of lca) (v_of a) (v_of b) =
+         seq_foldl do (v_of lca) (ops_of a) /\
+         (exists l. is_interleaving l (ops_of a) (ops_of b) /\
+               v_of (linearized_merge (v_of lca) l) == concrete_merge (v_of lca) (v_of a) (v_of b)))
+  = lem_inverse a;
+    assert (is_interleaving (ops_of a) (ops_of a) (ops_of b)); ()
+
+
+// length of branch b is > 0 and branch a is 0
+let linearizable_b_gt0 (lca a b:st)
+  : Lemma
+      (requires 
+         length (ops_of a) = 0 /\ length (ops_of b) <> 0 /\
+         v_of lca == init_of a /\
+         init_of a == init_of b)
+      (ensures 
+         concrete_merge_pre (v_of lca) (v_of a) (v_of b) /\
+         concrete_merge (v_of lca) (v_of a) (v_of b) =
+         seq_foldl do (v_of lca) (ops_of b) /\
+         (exists l. is_interleaving l (ops_of a) (ops_of b) /\
+               v_of (linearized_merge (v_of lca) l) == concrete_merge (v_of lca) (v_of a) (v_of b)))
+  = lem_inverse b;
+    assert (is_interleaving (ops_of b) (ops_of a) (ops_of b)); ()
+
+
+// length of both branches is 0
+let linearizable_ab_0 (lca a b:st)
+  : Lemma
+      (requires 
+         length (ops_of a) = 0 /\ length (ops_of b) = 0 /\
+         v_of lca == init_of a /\
+         init_of a == init_of b)
+      (ensures 
+         concrete_merge (v_of lca) (v_of a) (v_of b) = v_of lca /\
+         (exists l. is_interleaving l (ops_of a) (ops_of b) /\
+               v_of (linearized_merge (v_of lca) l) == concrete_merge (v_of lca) (v_of a) (v_of b)))
+  = assert (is_interleaving empty (ops_of a) (ops_of b)); ()
+
+
+#set-options "--initial_fuel 0 --max_fuel 2 --initial_ifuel 0 --max_ifuel 2 --z3rlimit 2000"
+let rec linearizable (lca s1 s2:st)
+  : Lemma 
+      (requires 
+         v_of lca == init_of s1 /\
+         init_of s1 == init_of s2 (*)/\
+         distinct_ops (ops_of lca ++ (ops_of s1 ++ ops_of s2)*))
+      (ensures 
+         (exists l. is_interleaving l (ops_of s1) (ops_of s2) /\
+         concrete_merge_pre (v_of lca) (v_of s1) (v_of s2) /\
+         v_of (linearized_merge (v_of lca) l) == concrete_merge (v_of lca) (v_of s1) (v_of s2)))
+      (decreases %[length (ops_of s1); length (ops_of s2)])
+
+  = match length (ops_of s1), length (ops_of s2) with
+    |0,0 -> linearizable_ab_0 lca s1 s2
+    |0,_ -> linearizable_b_gt0 lca s1 s2
+    |_,0 -> linearizable_a_gt0 lca s1 s2
+    |_,_ -> linearizable_ab_gt0 lca s1 s2;
+           linearizable lca (seq_foldl do (init_of s1) (fst (un_snoc (ops_of s1))), 
+                             hide (init_of s1, (fst (un_snoc (ops_of s1)))))
+                            (seq_foldl do (init_of s2) (fst (un_snoc (ops_of s2))), 
+                             hide (init_of s2, (fst (un_snoc (ops_of s2)))))
